code/blake2/Hacl.Impl.Blake2.Core.fst
@@ -1,0 +1,351 @@
+module Hacl.Impl.Blake2.Core
+module ST = FStar.HyperStack.ST
+open FStar.HyperStack
+open FStar.HyperStack.All
+open FStar.Mul
+
+open Lib.IntTypes
+open Lib.Buffer
+open Lib.ByteBuffer
+open Lib.IntVector
+
+module Spec = Spec.Blake2_Vec
+
+type m_spec =
+  | M32
+  | M128
+  | M256
+
+inline_for_extraction
+unfold type word_t (a:Spec.alg) = Spec.word_t a
+
+inline_for_extraction
+unfold let element_t (a:Spec.alg) (m:m_spec) =
+  match a,m with
+  | Spec.Blake2S,M128 -> (vec_t U32 4)
+  | Spec.Blake2S,M256 -> (vec_t U32 4)
+  | Spec.Blake2B,M256 -> (vec_t U64 4)
+  | _ -> (word_t a)
+
+inline_for_extraction
+unfold let zero_element (a:Spec.alg) (m:m_spec) : element_t a m =
+  match a,m with
+  | Spec.Blake2S,M128 -> (vec_zero U32 4)
+  | Spec.Blake2S,M256 -> (vec_zero U32 4)
+  | Spec.Blake2B,M256 -> (vec_zero U64 4)
+  | _ -> Spec.zero a
+
+inline_for_extraction
+unfold let row_len (a:Spec.alg) (m:m_spec) : size_t =
+  match a,m with
+  | Spec.Blake2S,M128 -> 1ul
+  | Spec.Blake2S,M256 -> 1ul
+  | Spec.Blake2B,M256 -> 1ul
+  | _ -> 4ul
+
+inline_for_extraction
+unfold let row_p (a:Spec.alg) (m:m_spec) =
+  lbuffer (element_t a m) (row_len a m)
+
+inline_for_extraction
+val row_v: #a:Spec.alg -> #m:m_spec -> h:mem -> row_p a m -> GTot (Spec.row a)
+inline_for_extraction
+let row_v #a #m h r =
+  match a,m with
+  | Spec.Blake2S,M128 -> vec_v (Lib.Sequence.index (as_seq h r) 0)
+  | Spec.Blake2S,M256 -> vec_v (Lib.Sequence.index (as_seq h r) 0)
+  | Spec.Blake2B,M256 -> vec_v (Lib.Sequence.index (as_seq h r) 0)
+  | _ -> as_seq h r
+
+noextract
+val row_v_lemma: #a:Spec.alg -> #m:m_spec -> h0:mem -> h1:mem -> r:row_p a m ->
+  Lemma (ensures (as_seq h0 r == as_seq h1 r ==>
+		  row_v h0 r == row_v h1 r))
+	[SMTPat (row_v h0 r); SMTPat (row_v h1 r)]
+let row_v_lemma #a #m h0 h1 r = ()
+
+inline_for_extraction
+unfold let state_p (a:Spec.alg) (m:m_spec) =
+  lbuffer (element_t a m) (4ul *. row_len a m)
+
+inline_for_extraction
+unfold let index_t = n:size_t{v n < 4}
+
+inline_for_extraction
+let g_rowi (#a:Spec.alg) (#m:m_spec) (st:state_p a m)  (idx:index_t) : GTot (row_p a m) =
+  gsub st (idx *. row_len a m) (row_len a m)
+
+#push-options "--z3rlimit  50"
+val g_rowi_disjoint: #a:Spec.alg -> #m:m_spec -> st:state_p a m -> idx1:index_t -> idx2:index_t ->
+  Lemma (ensures (idx1 <> idx2 ==> disjoint (g_rowi st idx1) (g_rowi st idx2)))
+	[SMTPat (disjoint (g_rowi st idx1) (g_rowi st idx2))]
+let g_rowi_disjoint #a #m st idx1 idx2 =
+  if idx1 <. idx2 then (
+    assert (v (idx1 *. row_len a m) + v (row_len a m) <= v (idx2 *. row_len a m));
+    assert (g_rowi st idx1 ==
+	    gsub st (idx1 *. row_len a m) (row_len a m));
+    assert (g_rowi st idx2 ==
+	    gsub st (idx2 *. row_len a m) (row_len a m));
+   LowStar.Monotonic.Buffer.loc_disjoint_gsub_buffer #_ #((LowStar.Buffer.trivial_preorder (element_t a m))) #((LowStar.Buffer.trivial_preorder (element_t a m))) st (idx1 *. row_len a m) (row_len a m) (LowStar.Buffer.trivial_preorder (element_t a m)) (idx2 *. row_len a m) (row_len a m) (LowStar.Buffer.trivial_preorder (element_t a m))
+    )
+  else if idx2 <. idx1 then (
+    assert (v (idx2 *. row_len a m) + v (row_len a m) <= v (idx1 *. row_len a m));
+    assert (g_rowi st idx2 ==
+	    gsub st (idx2 *. row_len a m) (row_len a m));
+    LowStar.Monotonic.Buffer.loc_disjoint_gsub_buffer #_ #((LowStar.Buffer.trivial_preorder (element_t a m))) #((LowStar.Buffer.trivial_preorder (element_t a m))) st (idx1 *. row_len a m) (row_len a m) (LowStar.Buffer.trivial_preorder (element_t a m)) (idx2 *. row_len a m) (row_len a m) (LowStar.Buffer.trivial_preorder (element_t a m)))
+  else ()
+
+val g_rowi_unchanged: #a:Spec.alg -> #m:m_spec -> h0:mem -> h1:mem -> st:state_p a m -> i:index_t ->
+  Lemma (requires (as_seq h0 st == as_seq h1 st))
+	(ensures (as_seq h0 (g_rowi st i) == as_seq h1 (g_rowi st i)))
+	[SMTPat (as_seq h0 (g_rowi st i)); SMTPat (as_seq h1 (g_rowi st i))]
+let g_rowi_unchanged #a #m h0 h1 st i =
+  assert (v (i *. row_len a m) + v (row_len a m) <= length st);
+  LowStar.Monotonic.Buffer.as_seq_gsub #_ #(LowStar.Buffer.trivial_preorder (element_t a m)) #(LowStar.Buffer.trivial_preorder (element_t a m)) h0 st (i *. row_len a m) (row_len a m)
+  (LowStar.Buffer.trivial_preorder (element_t a m));
+  LowStar.Monotonic.Buffer.as_seq_gsub #_ #(LowStar.Buffer.trivial_preorder (element_t a m)) #(LowStar.Buffer.trivial_preorder (element_t a m)) h1 st (i *. row_len a m) (row_len a m)
+  (LowStar.Buffer.trivial_preorder (element_t a m))
+
+val g_rowi_disjoint_other:  #a:Spec.alg -> #m:m_spec -> #b:Type -> #len:size_t -> st:state_p a m -> i:index_t -> x:lbuffer b len ->
+  Lemma(requires (disjoint st x))
+       (ensures (disjoint (g_rowi st i) x /\ disjoint x (g_rowi st i)))
+let g_rowi_disjoint_other #a #m #b #len st i x =
+  assert (v (i *. row_len a m) + v (row_len a m) <= length st);
+    LowStar.Monotonic.Buffer.loc_includes_gsub_buffer_r'  #_ #(LowStar.Buffer.trivial_preorder (element_t a m)) #(LowStar.Buffer.trivial_preorder (element_t a m)) st (i *. row_len a m) (row_len a m)
+  (LowStar.Buffer.trivial_preorder (element_t a m))
+#pop-options
+
+inline_for_extraction
+let state_v (#a:Spec.alg) (#m:m_spec) (h:mem) (st:state_p a m) : GTot (Spec.state a) =
+  let r0 = row_v h (g_rowi st 0ul) in
+  let r1 = row_v h (g_rowi st 1ul) in
+  let r2 = row_v h (g_rowi st 2ul) in
+  let r3 = row_v h (g_rowi st 3ul) in
+  create4 r0 r1 r2 r3
+
+noextract
+val state_v_lemma: #a:Spec.alg -> #m:m_spec -> h0:mem -> h1:mem -> st:state_p a m ->
+  Lemma (requires (as_seq h0 st == as_seq h1 st))
+	(ensures (state_v h0 st == state_v h1 st))
+	[SMTPat (state_v h0 st); SMTPat (state_v h1 st)]
+let state_v_lemma #a #m h0 h1 st = ()
+
+
+#push-options "--z3rlimit 50"
+val modifies_row: a:Spec.alg -> m:m_spec -> h0:mem -> h1:mem -> st:state_p a m -> i:index_t ->
+  Lemma (requires (live h0 st /\ modifies (loc (g_rowi st i)) h0 h1))
+	(ensures (state_v h1 st == Lib.Sequence.((state_v h0 st).[v i] <- row_v h1 (g_rowi st i))))
+	[SMTPat (modifies (loc (g_rowi st i)) h0 h1)]
+let modifies_row a m h0 h1 st i =
+    assert (live h0 (g_rowi st 0ul));
+    assert (live h0 (g_rowi st 1ul));
+    assert (live h0 (g_rowi st 2ul));
+    assert (live h0 (g_rowi st 3ul));
+    Lib.Sequence.(eq_intro (state_v h1 st) ((state_v h0 st).[v i] <- row_v h1 (g_rowi st i)))
+#pop-options
+
+
+inline_for_extraction
+val rowi: #a:Spec.alg -> #m:m_spec -> st:state_p a m -> idx:index_t ->
+	  ST (row_p a m)
+	  (requires (fun h -> live h st))
+	  (ensures (fun h0 r h1 -> h0 == h1 /\ live h1 r /\ r == g_rowi st idx))
+
+inline_for_extraction
+let rowi (#a:Spec.alg) (#m:m_spec) (st:state_p a m)  (idx:index_t) =
+  sub st (idx *. row_len a m) (row_len a m)
+
+
+inline_for_extraction
+val xor_row: #a:Spec.alg -> #m:m_spec -> r1:row_p a m -> r2:row_p a m ->
+	  ST unit
+	  (requires (fun h -> live h r1 /\ live h r2 /\ disjoint r1 r2))
+	  (ensures (fun h0 _ h1 -> modifies (loc r1) h0 h1 /\
+				row_v h1 r1 == Spec.( row_v h0 r1 ^| row_v h0 r2 )))
+inline_for_extraction
+let xor_row #a #m r1 r2 =
+  match a,m with
+  | Spec.Blake2S,M128 ->
+    r1.(0ul) <- vec_xor #U32 #4 r1.(0ul) r2.(0ul)
+  | Spec.Blake2S,M256 ->
+    r1.(0ul) <- vec_xor #U32 #4 r1.(0ul) r2.(0ul)
+  | Spec.Blake2B,M256 ->
+    r1.(0ul) <- vec_xor #U64 #4 r1.(0ul) r2.(0ul)
+  | _ -> map2T 4ul r1 (logxor #(Spec.wt a) #SEC) r1 r2
+
+
+inline_for_extraction
+val add_row: #a:Spec.alg -> #m:m_spec -> r1:row_p a m -> r2:row_p a m ->
+	  ST unit
+	  (requires (fun h -> live h r1 /\ live h r2 /\ disjoint r1 r2))
+	  (ensures (fun h0 _ h1 -> modifies (loc r1) h0 h1 /\
+				row_v h1 r1 == Spec.( row_v h0 r1 +| row_v h0 r2 )))
+inline_for_extraction
+let add_row #a #m r1 r2 =
+  match a,m with
+  | Spec.Blake2S,M128 ->
+    r1.(0ul) <- vec_add_mod #U32 #4 r1.(0ul) r2.(0ul)
+  | Spec.Blake2S,M256 ->
+    r1.(0ul) <- vec_add_mod #U32 #4 r1.(0ul) r2.(0ul)
+  | Spec.Blake2B,M256 ->
+    r1.(0ul) <- vec_add_mod #U64 #4 r1.(0ul) r2.(0ul)
+  | _ -> map2T 4ul r1 (add_mod #(Spec.wt a) #SEC) r1 r2
+
+
+inline_for_extraction
+val ror_row: #a:Spec.alg -> #m:m_spec -> r1:row_p a m -> r2:rotval (Spec.wt a) ->
+	  ST unit
+	  (requires (fun h -> live h r1))
+	  (ensures (fun h0 _ h1 -> modifies (loc r1) h0 h1 /\
+				row_v h1 r1 == Spec.( row_v h0 r1 >>>| r2 )))
+inline_for_extraction
+let ror_row #a #m r1 r2 =
+  match a,m with
+  | Spec.Blake2S,M128 ->
+    r1.(0ul) <- vec_rotate_right #U32 #4 r1.(0ul) r2
+  | Spec.Blake2S,M256 ->
+    r1.(0ul) <- vec_rotate_right #U32 #4 r1.(0ul) r2
+  | Spec.Blake2B,M256 ->
+    r1.(0ul) <- vec_rotate_right #U64 #4 r1.(0ul) r2
+  | _ ->
+    let r1:lbuffer (Spec.word_t a) 4ul = r1 in
+    mapT 4ul r1 (rotate_right_i #(Spec.wt a) #SEC r2) r1
+
+
+inline_for_extraction
+val permr_row: #a:Spec.alg -> #m:m_spec -> r1:row_p a m -> n:index_t ->
+	  ST unit
+	  (requires (fun h -> live h r1))
+	  (ensures (fun h0 _ h1 -> modifies (loc r1) h0 h1 /\
+				row_v h1 r1 == Spec.( rotr (row_v h0 r1) (v n) )))
+
+#push-options "--z3rlimit 50"
+inline_for_extraction
+let permr_row #a #m r1 n =
+  let n0,n1,n2,n3 = n,(n+.1ul)%.4ul,(n+.2ul)%.4ul,(n+.3ul)%.4ul in
+  match a,m with
+  | Spec.Blake2S,M256
+  | Spec.Blake2S,M128 ->
+    let v0 : vec_t U32 4 = r1.(0ul) in
+    let v1 : vec_t U32 4 = vec_permute4 #U32 v0 n0 n1 n2 n3 in
+    Lib.Sequence.(eq_intro (create4 (vec_v v0).[v n0] (vec_v v0).[v n1] (vec_v v0).[v n2] (vec_v v0).[v n3]) (Lib.Sequence.(createi 4 (fun i -> (vec_v v0).[(i+v n)%4]))));
+    Lib.Sequence.(eq_intro (Spec.rotr (vec_v v0) (v n)) (Lib.Sequence.(createi 4 (fun i -> (vec_v v0).[(i+v n)%4]))));
+    r1.(0ul) <- v1
+  | Spec.Blake2B,M256 ->
+    let v0 : vec_t U64 4 = r1.(0ul) in
+    let v1 : vec_t U64 4 = vec_permute4 #U64 v0 n0 n1 n2 n3 in
+    Lib.Sequence.(eq_intro (create4 (vec_v v0).[v n0] (vec_v v0).[v n1] (vec_v v0).[v n2] (vec_v v0).[v n3]) (Lib.Sequence.(createi 4 (fun i -> (vec_v v0).[(i+v n)%4]))));
+    Lib.Sequence.(eq_intro (Spec.rotr (vec_v v0) (v n)) (Lib.Sequence.(createi 4 (fun i -> (vec_v v0).[(i+v n)%4]))));
+    r1.(0ul) <- v1
+  | _ ->
+    let h0 = ST.get() in
+    let r1:lbuffer (Spec.word_t a) 4ul = r1 in
+    let x0 = r1.(n0) in
+    let x1 = r1.(n1) in
+    let x2 = r1.(n2) in
+    let x3 = r1.(n3) in
+    r1.(0ul) <- x0;
+    r1.(1ul) <- x1;
+    r1.(2ul) <- x2;
+    r1.(3ul) <- x3;
+    let h1 = ST.get() in
+    Lib.Sequence.(let s0 = as_seq h0 r1 in eq_intro (create4 x0 x1 x2 x3) (createi 4 (fun i -> s0.[(i+v n)%4])));
+    Lib.Sequence.(let s0 = as_seq h0 r1 in eq_intro (Spec.rotr s0 (v n)) (Lib.Sequence.(createi 4 (fun i -> s0.[(i+v n)%4]))));
+    Lib.Sequence.(eq_intro (as_seq h1 r1) (create4 x0 x1 x2 x3));
+    ()
+#pop-options
+
+#push-options "--z3rlimit 50"
+val create4_lemma: #a:Type -> x0:a -> x1:a -> x2:a -> x3:a ->
+  Lemma (ensures (Lib.Sequence.createL [x0;x1;x2;x3] == create4 x0 x1 x2 x3))
+	[SMTPat (Lib.Sequence.createL [x0;x1;x2;x3])]
+let create4_lemma #a x0 x1 x2 x3 =
+  let open Lib.Sequence in
+  let l : list a = [x0;x1;x2;x3] in
+  assert_norm (List.Tot.index l 0 == x0);
+  assert_norm (List.Tot.index l 1 == x1);
+  assert_norm (List.Tot.index l 2 == x2);
+  assert_norm (List.Tot.index l 3 == x3);
+  let s1 : lseq a 4 = of_list l in
+  let s2 : lseq a 4 = create4 x0 x1 x2 x3 in
+  eq_intro s1 s2
+#pop-options
+
+inline_for_extraction
+val alloc_row: a:Spec.alg -> m:m_spec ->
+	  StackInline (row_p a m)
+	  (requires (fun h -> True))
+	  (ensures (fun h0 r h1 -> stack_allocated r h0 h1 (Lib.Sequence.create (v (row_len a m)) (zero_element a m)) /\
+				live h1 r /\
+				row_v h1 r == Spec.zero_row a))
+
+inline_for_extraction
+let alloc_row a m = create (row_len a m) (zero_element a m)
+
+
+inline_for_extraction
+val create_row: #a:Spec.alg -> #m:m_spec -> r1:row_p a m -> w0:word_t a -> w1:word_t a -> w2:word_t a -> w3:word_t a ->
+	  ST unit
+	  (requires (fun h -> live h r1))
+	  (ensures (fun h0 _ h1 -> modifies (loc r1) h0 h1 /\
+				row_v h1 r1 == Spec.( create_row w0 w1 w2 w3 )))
+
+inline_for_extraction
+let create_row #a #m r w0 w1 w2 w3 =
+  match a,m with
+  | Spec.Blake2S,M256
+  | Spec.Blake2S,M128
+  | Spec.Blake2B,M256 ->
+    r.(0ul) <- vec_load4 w0 w1 w2 w3
+  | _ ->
+    r.(0ul) <- w0;
+    r.(1ul) <- w1;
+    r.(2ul) <- w2;
+    r.(3ul) <- w3;
+    let h1 = ST.get() in
+    Lib.Sequence.eq_intro (as_seq h1 r) (create4 w0 w1 w2 w3)
+
+inline_for_extraction
+val load_row: #a:Spec.alg -> #m:m_spec -> r1:row_p a m -> ws:lbuffer (word_t a) 4ul ->
+	  ST unit
+	  (requires (fun h -> live h r1 /\ live h ws /\ disjoint r1 ws))
+	  (ensures (fun h0 _ h1 -> modifies (loc r1) h0 h1 /\
+				row_v h1 r1 == Spec.( load_row (as_seq h0 ws))))
+
+inline_for_extraction
+let load_row #a #m r ws = create_row r ws.(0ul) ws.(1ul) ws.(2ul) ws.(3ul)
+
+inline_for_extraction
+val gather_row: #a:Spec.alg -> #ms:m_spec -> #len:size_t -> r:row_p a ms -> m:lbuffer uint8 len ->
+          i0: Spec.word_index a (v len) -> i1:Spec.word_index a (v len) -> i2:Spec.word_index a (v len) -> i3:Spec.word_index a (v len)
+	  -> ST unit
+	  (requires (fun h -> live h r /\ live h m /\ disjoint r m))
+	  (ensures (fun h0 _ h1 -> modifies (loc r) h0 h1 /\
+				row_v h1 r == Spec.( gather_row (as_seq h0 m) i0 i1 i2 i3)))
+
+#push-options "--z3rlimit 100"
+inline_for_extraction
+let gather_row #a #ms #len r m i0 i1 i2 i3 =
+  let h0 = ST.get() in
+  let nb = size (Spec.size_word a) in
+  let b0 = sub m (i0 *. nb) nb in
+  let b1 = sub m (i1 *. nb) nb in
+  let b2 = sub m (i2 *. nb) nb in
+  let b3 = sub m (i3 *. nb) nb in
+  as_seq_gsub h0 m (i0 *. nb) nb;
+  as_seq_gsub h0 m (i1 *. nb) nb;
+  as_seq_gsub h0 m (i2 *. nb) nb;
+  as_seq_gsub h0 m (i3 *. nb) nb;
+  assert (as_seq h0 b0 == Lib.Sequence.sub (as_seq h0 m) (v i0 * Spec.size_word a) (Spec.size_word a));
+  assert (as_seq h0 b1 == Lib.Sequence.sub (as_seq h0 m) (v i1 * Spec.size_word a) (Spec.size_word a));
+  assert (as_seq h0 b2 == Lib.Sequence.sub (as_seq h0 m) (v i2 * Spec.size_word a) (Spec.size_word a));
+  assert (as_seq h0 b3 == Lib.Sequence.sub (as_seq h0 m) (v i3 * Spec.size_word a) (Spec.size_word a));
+  let u0 = uint_from_bytes_le #(Spec.wt a) b0 in
+  let u1 = uint_from_bytes_le #(Spec.wt a) b1 in
+  let u2 = uint_from_bytes_le #(Spec.wt a) b2 in
+  let u3 = uint_from_bytes_le #(Spec.wt a) b3 in
+  assert (u0 == Lib.ByteSequence.uint_from_bytes_le (as_seq h0 b0));
+  create_row r u0 u1 u2 u3
+#pop-options
+
+  
